Added missing proofs from previous commit.

realizability/Realizability.v
@@ -1,3 +1,8 @@
+Definition admit {T: Type} : T.  Admitted.
+
+(* --- Towards Realizability Checking of Contracts using Theories --- *)
+(* --- Machine-Checked Proofs For Realizability Checking Algorithms --- *)
+
 Inductive id : Type :=
 Id : nat -> id.
 
@@ -17,70 +22,59 @@ Definition tguarantee := state -> inputs -> state -> Prop.
 
 Definition assumption := state -> inputs -> Prop.
 
-Inductive reachable (s : state) (init : initial) (t : transition) (a : assumption) : Prop :=
-rch : ((init s) \/
-      (exists (s' : state) (inp : inputs),(reachable s' init t a) /\ (a s' inp) /\ (t s' inp s))) ->
+Inductive reachable (s:state) (init: initial) (t: transition) (a:assumption) : Prop :=
+rch : ((init s) \/ (exists (s':state) (inp:inputs), 
+                          (reachable s' init t a) /\ (a s' inp) /\ (t s' inp s))) ->
        reachable s init t a.
 
-Inductive realization (init : initial) (t : transition) (a : assumption) (gi : iguarantee) (gt : tguarantee) : Prop :=
-real : ((forall (s : state), (init s) -> (gi s)) /\
-       (forall (s s' : state) (inp : inputs), 
+Inductive realization (init : initial) (t : transition) (a:assumption) (gi:iguarantee) (gt: tguarantee) : Prop :=
+real : ((forall (s:state), (init s) -> (gi s)) /\
+       (forall (s s':state) (inp : inputs), 
           ((reachable s init t a) /\ (a s inp) /\ (t s inp s')) -> gt s inp s') /\
-       (exists (s : state), init s) /\
-       (forall (s : state) (inp:inputs), (reachable s init t a /\ (a s inp)) -> 
-         (exists (s' : state), t s inp s'))) ->
+       (exists (s:state), init s) /\
+       (forall (s:state) (inp:inputs), (reachable s init t a /\ (a s inp)) -> 
+         (exists (s':state), t s inp s')))->
        realization init t a gi gt.
 
-Inductive realizable_contract (a : assumption) (gi : iguarantee) (gt : tguarantee) : Prop :=
+Inductive realizable_contract (a:assumption) (gi: iguarantee) (gt: tguarantee) : Prop :=
 rc : (exists (init : initial) (t : transition), realization init t a gi gt) -> realizable_contract a gi gt.
 
-CoInductive viable (s : state) (a : assumption) (gi : iguarantee) (gt : tguarantee) : Prop :=
-vbl : (forall (i : inputs), (a s i) -> (exists (s' : state), gt s i s' /\ viable s' a gi gt)) -> viable s a gi gt.
+CoInductive viable (s:state) (a:assumption) (gi:iguarantee) (gt: tguarantee) : Prop :=
+vbl : (forall (i:inputs), (a s i) -> (exists (s':state), gt s i s' /\ viable s' a gi gt)) -> viable s a gi gt.
 
-Inductive realizable (a : assumption) (gi : iguarantee) (gt : tguarantee) : Prop :=
-rl : (exists (s : state), gi s /\ viable s a gi gt) -> realizable a gi gt.
+Inductive realizable (a:assumption) (gi : iguarantee) (gt:tguarantee) : Prop :=
+rl : (exists (s:state), gi s /\ viable s a gi gt) -> realizable a gi gt.
 
 
-Lemma init_reachable : forall (s:state) (init : initial) (t : transition) (a : assumption),
+Lemma init_reachable : forall (s:state) (init:initial) (t:transition) (a:assumption),
 init s -> reachable s init t a.
 Proof. intros. apply rch. left. apply H. Qed.
 
 
-Lemma reachable_viable : forall (s : state) (init : initial) (t : transition) (a : assumption) (gi : iguarantee) (gt : tguarantee),
+Lemma reachable_viable : forall (s :state) (init:initial) (t:transition) (a:assumption) (gi:iguarantee) (gt:tguarantee),
 realization init t a gi gt -> reachable s init t a -> viable s a gi gt.
 
-Proof. cofix. intros. apply vbl. intros. inversion H.
-inversion H2. inversion H4. inversion H6. destruct H8 with (s:=s) (inp:=i). 
-  split.
-    apply H0. apply H1. exists x. split.
-      apply H5. split.
-        apply H0. split.
-          apply H1.
-          apply H9.
-      apply reachable_viable with (init:= init) (t:=t). 
-        apply H.
-        apply rch. right. exists s. exists i. split.
-          apply H0. split.
-            apply H1. 
-            apply H9.
+Proof. cofix. intros. apply vbl. intros. inversion H. inversion H2. inversion H4. inversion H6. destruct H8 with (s:=s) (inp:=i). split. apply H0. apply H1. exists x. split. apply H5.
+  split. apply H0. split. apply H1. apply H9. apply reachable_viable with (init:= init) (t:=t). apply H. apply rch. right. exists s. exists i. split. apply H0. split. apply H1. apply H9.
 Qed.
 
 
-Theorem realcontract_implies_real  (init : initial) (t : transition) : forall (a : assumption) (gi : iguarantee) (gt : tguarantee),
+Theorem realcontract_implies_real  (init:initial) (t:transition) : forall (a : assumption) (gi : iguarantee) (gt : tguarantee),
 realizable_contract a gi gt -> realizable a gi gt.
 Proof.
+  split.
   intros. apply rl. inversion H. inversion H0. inversion H1. inversion H2. inversion H3.
   inversion H5. inversion H7. inversion H8. exists x1. apply and_comm. split. apply init_reachable with (s:= x1) (t:=x0) (a:=a) in H10. apply reachable_viable with (gi:=gi) (gt:= gt) in H10. apply H10.
   apply H2. apply H4. apply H10.
 Qed.
 
-Theorem reach_via : forall (s s0 : state) (a : assumption) (gi : iguarantee) (gt : tguarantee),
+Theorem reach_via : forall (s s0:state) (a:assumption) (gi:iguarantee) (gt:tguarantee),
 viable s0 a gi gt -> reachable s (fun s => s = s0) (fun s i s' => gt s i s' /\ viable s' a gi gt) a -> viable s a gi gt.
 Proof.
   intros. inversion H0. inversion H1. subst. assumption. inversion H2. inversion H3. inversion H4. inversion H6. inversion H8. assumption.
 Qed.
 
-Theorem real_implies_realcontract (init : initial) (t : transition) : forall (a : assumption) (gi : iguarantee) (gt : tguarantee),
+Theorem real_implies_realcontract (init:initial) (t:transition) : forall (a : assumption) (gi : iguarantee) (gt : tguarantee),
 realizable a gi gt -> realizable_contract a gi gt.
 Proof.
   intros. apply rc. inversion H as [[s0 [gi_s0 viable_s0]]]. exists (fun s => s = s0).
@@ -95,108 +89,526 @@ Proof.
   intros. inversion H0. apply reach_via with (gi:=gi) (gt:=gt) in H1. inversion H1. apply H3. apply H2. assumption.
 Qed.
 
+Fixpoint finite_viable (n:nat) (s:state) (a:assumption) (gt:tguarantee) : Prop :=
+  match n with
+  | O => True
+  | S n' => forall i, a s i -> exists s', gt s i s' /\ finite_viable n' s' a gt
+  end.
 
-Inductive finite_viable : nat -> state -> assumption -> tguarantee -> Prop :=
-|fvnil : forall s a gt, finite_viable O s a gt
-|fv : forall m s a gt, finite_viable m s a gt -> (forall (i : inputs), a s i -> (exists s', gt s i s')) -> finite_viable (S m) s a gt.
+
+Fixpoint extendable (n:nat) (s:state) (a:assumption) (gt:tguarantee) : Prop :=
+  match n with
+  | O => forall i, a s i -> exists (s':state), gt s i s'
+  | S n' => forall i s', a s i -> gt s i s' -> extendable n' s' a gt
+  end.
+
+Definition Basecheck (n:nat) (a:assumption) (gi:iguarantee) (gt:tguarantee) :=
+exists (s:state), (gi s /\ finite_viable n s a gt).
 
 
-Inductive extendable : nat -> state -> assumption -> tguarantee -> Prop :=
-| exnil : forall s (a : assumption) gt, (forall i, a s i -> exists s', gt s i s') ->
-extendable O s a gt
-| ex : forall m s a gt, (forall i s', a s i /\ gt s i s' /\ extendable
-m s' a gt) -> extendable (S m) s a gt.
-
-Definition Basecheck (n : nat) (a : assumption) (gi : iguarantee) (gt : tguarantee) :=
-exists (s : state), (gi s /\ finite_viable n s a gt).
-
-Definition Extendcheck n (a : assumption) (gt : tguarantee) :=
+Definition Extendcheck (n:nat) (a:assumption) (gt:tguarantee) :=
 forall s a gt, extendable n s a gt.
 
-Lemma viable_implies_finite_viable : forall s a gi gt n,
+
+Lemma viable_implies_finite_viable : forall a gi gt n s,
 viable s a gi gt -> finite_viable n s a gt.
-Proof.
-  intros. induction n. simpl. intros.  inversion H. constructor.
-   inversion H. apply fv. apply IHn. intros. destruct H0 with (i:=i). assumption. exists x. inversion H2. assumption.
+Proof. intros a gi gt n. induction n. intros. simpl. auto.
+  intros. simpl. intros.  inversion H. apply H1 in H0.
+  inversion H0. inversion H2. exists x.
+  intros. split. apply H3. apply IHn. apply H4.
 Qed.
 
-Theorem unrealizable_soundness : forall (init : initial) (t : transition) a gi gt,
+Theorem unrealizable_soundness : forall (s:state) (init:initial) (t:transition) a gi gt,
 (exists n, ~Basecheck n a gi gt) -> ~ realizable_contract a gi gt.
 Proof.
   intros. unfold not. intros. apply realcontract_implies_real in H0. inversion H0. inversion H1. inversion H2. inversion H. apply viable_implies_finite_viable with (n:=x0) in H4.
   apply H5. unfold Basecheck. exists x. split. assumption. assumption. apply init. apply t.
 Qed.
 
-Lemma extend_viable_shift : forall (s : state) (n : nat) (i : inputs) (a : assumption) (gi : iguarantee) (gt : tguarantee),
-(extendable n s a gt /\ finite_viable n s a gt /\ a s i) -> (exists s', gt s i s' /\ finite_viable n s' a gt).
-Proof.
-  intros. induction n. inversion H. inversion H0. destruct H2 with (i:=i). inversion H1. assumption.
-  exists x. split. assumption. constructor.
+
+Lemma finite_viable_plus_one : forall n a gt (gi:iguarantee) (i:inputs) s,
+(extendable n s a gt /\ finite_viable n s a gt) -> finite_viable (S n) s a gt.
+Proof. intros n a gt gi i. induction n.
+  intros. simpl. intros. inversion H. simpl in H1. apply H1 in H0.
+  inversion H0. exists x. intros. auto.
   
-  inversion H. inversion H1. inversion H0. destruct H5 with (i:=i) (s':=s). exists s.
-  inversion H10. split. assumption. assumption.
+  intros. simpl. intros. inversion H. assert (H3: a s i0).
+  apply H0. simpl in H2. simpl in H1. apply H2 in H3. inversion H3.
+  exists x. intros. split. inversion H4. apply H5.
+  assert (H5: extendable n x a gt). apply H1 with (i:=i0).
+  apply H0. inversion H4. apply H5. inversion H4.
+  apply conj with (A:=extendable n x a gt) in H7.
+  apply IHn in H7. simpl in H7. intros. apply H7 in H8.
+  apply H8. apply H5.
 Qed.
 
-Lemma fv_ex_implies_viable : forall (s : state) n (a : assumption) gi gt,
+Lemma extend_viable_shift : forall (n : nat) (a : assumption) (gi : iguarantee) (gt : tguarantee) (s : state) (i : inputs),
+(extendable n s a gt /\ finite_viable n s a gt /\ a s i) -> (exists s', gt s i s' /\ finite_viable n s' a gt).
+Proof. intros n a gi gt. induction n.
+  intros. inversion H. simpl in H0. inversion H1.
+  apply H0 in H3. inversion H3. exists x. intros. simpl. auto.
+  
+  intros. inversion H. simpl in H0. inversion H1. assert (H4: a s i).
+  apply H3. simpl in H2. apply H2 in H3. inversion H3.
+  exists x. intros. simpl. intros.
+  assert (H8: a s i -> gt s i x -> extendable n x a gt).
+  apply H0. apply H8 in H4. inversion H5.
+  split. apply H6. intros. apply conj with (A:=extendable n x a gt) in H7.
+  apply finite_viable_plus_one in H7. simpl in H7. apply H7. apply H9.
+  apply gi. apply i. apply H4. inversion H5. apply H6.
+Qed.
+
+Lemma fv_ex_implies_viable : forall n (a:assumption) gi gt (init:initial) (t:transition) (s:state),
 (finite_viable n s a gt /\ Extendcheck n a gt) -> viable s a gi gt.
 Proof.
- cofix. intros. apply vbl. inversion H. unfold Extendcheck in H1.
- intros. apply conj with (A:= finite_viable n s a gt) in H2.
- apply conj with (A:= extendable n s a gt) in H2.
- apply extend_viable_shift in H2. destruct H2.
- inversion H2. exists x. split. assumption.
- apply fv_ex_implies_viable with (n:=n).
- split. assumption. unfold Extendcheck. assumption.
- apply gi. apply H1. inversion H. assumption.
+ cofix. intros n a gi gt init t. intros. apply vbl.
+ intros. inversion H. unfold Extendcheck in H2.
+ assert (H3: extendable n s a gt). apply H2.
+ apply conj with (A:=finite_viable n s a gt) in H0.
+ apply conj with (A:= extendable n s a gt) in H0.
+ apply extend_viable_shift in H0. inversion H0.
+ exists x. inversion H4. split. apply H5.
+ apply fv_ex_implies_viable with (n:=n). apply init.
+ apply t. split. apply H6. inversion H. apply H8.
+ apply gi.  apply H3. apply H1.
 Qed.
 
-Theorem realizable_soundness : forall (init : initial) (t : transition) a gi gt,
+Theorem realizable_soundness : forall (s:state) (init:initial) (t:transition) a gi gt,
 (exists n, (Basecheck n a gi gt /\ Extendcheck n a gt)) -> realizable_contract a gi gt.
 Proof.
   intros. apply real_implies_realcontract. apply init. apply t. apply rl.
-  inversion H. inversion H0. inversion H1. inversion H3.
-  exists x0. split. assumption. apply fv_ex_implies_viable with (n:=x). split.
+  inversion H. inversion H0. inversion H1. subst. inversion H3. unfold Basecheck in H4.
+  exists x0. split. assumption. apply fv_ex_implies_viable with (n:=x). apply gi. apply t. split.
   assumption. assumption.
 Qed.
 
-Lemma finite_viable_plus_one : forall s n a gt (gi : iguarantee) (i : inputs),
-(extendable n s a gt /\ finite_viable n s a gt) -> finite_viable (S n) s a gt.
-Proof.
-  intros. induction n. apply fv. constructor. inversion H. inversion H0.
-  intros. apply H2 in H3. assumption.
-
-  apply fv. apply IHn. split. inversion H. inversion H0.
-  destruct H3 with (i:=i) (s':=s). inversion H8. assumption.
-  inversion H. inversion H1. assumption.
-  intros. inversion H.
-  inversion H2. apply H5 in H0. apply H0.
-Qed.
-
-Definition Basecheck_simple (n : nat) (a : assumption) (gi : iguarantee) (gt : tguarantee):=
+Definition Basecheck_simple (n:nat) (a:assumption) (gi:iguarantee) (gt:tguarantee):=
 forall s, (gi s) -> extendable n s a gt.
 
-Theorem basecheck_soundness_one_way : forall n a (gi : iguarantee) gt (i : inputs),
+Theorem basecheck_soundness_one_way : forall n a (gi:iguarantee) gt (i:inputs),
 ((exists s, gi s) /\
 (forall k, (k<=n) -> Basecheck_simple k a gi gt)) -> Basecheck n a gi gt.
 Proof.
-  intros. induction n. inversion H. inversion H0. unfold Basecheck. exists x. split. assumption. constructor.
+  intros. induction n. unfold Basecheck. assert (H0: 0<=0). apply le_n. 
+  inversion H. inversion H1. exists x. split. assumption. constructor.
 
   unfold Basecheck. inversion H.
   assert (H3: (forall k : nat, k <= n -> Basecheck_simple k a gi gt)).
-  intros. apply le_S in H2. apply H1. assumption.
-  apply conj with (A:= exists s : state, gi s) in H3.
+  intros. apply le_S in H2. inversion H. apply H4 in H2.
+  assumption. apply conj with (A:= exists s : state, gi s) in H3.
   apply IHn in H3. inversion H3. inversion H2.
   exists x. split. assumption.
   
-  apply finite_viable_plus_one. apply gi. apply i. split. unfold Basecheck_simple in H1.
+  apply finite_viable_plus_one. assumption. assumption. split. unfold Basecheck_simple in H1.
   apply H1. apply le_S. apply le_n. assumption. assumption.
   assumption.
 Qed.
 
-Definition witness (i:inputs) (n:nat) (s:state) (a:assumption) (gi: iguarantee) (gt: tguarantee) :=
-forall i s k n, (k<=n -> (a s i) /\ exists s', gt s i s') /\ extendable (S n) s a gt.
+(* --- Synthesis from Assume-Guarantee Contracts using Skolemized Proofs of Realizability --- *)
 
-Theorem asd : forall i n a gi gt, (Basecheck n a gi gt /\ Extendcheck n a gt) -> exists s, witness i n s a gi gt.
-intros.
-  inversion H. inversion H0. exists x. inversion H2. assert (H5: extendable n x a gt). apply H1. unfold witness.
-  intros. split. intros.
+Definition skolem_0 (s:state) (i:inputs) : state := admit.
+Definition skolem_1 (s:state) (i: inputs) (s': state) (i': inputs) : state := admit.
+
+Inductive extendable_f : nat -> state -> assumption -> tguarantee -> Prop :=
+|exnill : forall s (a:assumption) (gt:tguarantee), (forall i, a s i -> (gt s i (skolem_0 s i))) ->
+extendable_f O s a gt
+|exone : forall s i (a:assumption) (gt:tguarantee), a s i /\ gt s i (skolem_0 s i) /\ 
+   (forall s' i', a s' i' -> gt s' i' (skolem_1 s i s' i')) -> extendable_f (S O) s a gt.
+
+
+Theorem extf_zero_implies_ext_zero : forall (a:assumption) (gt:tguarantee) (s:state),
+extendable_f O s a gt -> extendable O s a gt.
+Proof.
+  intros n a gt.
+  intros. inversion H. simpl. intros. exists (skolem_0 s i).
+  apply H0. apply H1.
+Qed.
+
+Theorem extf_one_implies_ext_one : forall (a:assumption) (gt:tguarantee) (s:state),
+extendable_f 1 s a gt -> extendable 1 s a gt.
+Proof.
+  intros. simpl. intros. inversion H. inversion H3. inversion H8.
+  assert (H11: gt s' i0 (skolem_1 s i1 s' i0)).
+  apply H10. apply H2.  exists (skolem_1 s i1 s' i0).  apply H11. 
+Qed.
+
+Definition Basecheck_simple_f (n:nat) (a:assumption) (gi:iguarantee) (gt:tguarantee):=
+forall s, (gi s) -> extendable_f n s a gt.
+
+Definition Extendcheck_f (n:nat) (a:assumption) (gt:tguarantee) :=
+forall s a gt, extendable_f n s a gt.
+
+Theorem BCheck_f_imp_BCheck_zero : forall (a:assumption) (gi:iguarantee) (gt:tguarantee),
+Basecheck_simple_f O a gi gt -> Basecheck_simple O a gi gt.
+Proof.
+  intros. unfold Basecheck_simple_f in H. unfold Basecheck_simple.
+  intros. apply extf_zero_implies_ext_zero. apply H. apply H0.
+Qed.
+
+Theorem BCheck_f_imp_BCheck_one : forall (a:assumption) (gi:iguarantee) (gt:tguarantee),
+Basecheck_simple_f 1 a gi gt -> Basecheck_simple 1 a gi gt.
+Proof.
+  intros. unfold Basecheck_simple_f in H. unfold Basecheck_simple.
+  intros. apply H in H0. simpl. intros. inversion H0. inversion H4. inversion H9.
+  assert (H12: gt s' i0 (skolem_1 s i1 s' i0)). apply H11. assumption.
+  exists (skolem_1 s i1 s' i0). apply H12.
+Qed.
+
+Theorem ECheck_f_imp_ECheck_zero : forall (a:assumption) (gt:tguarantee) (s:state),
+Extendcheck_f O a gt -> Extendcheck O a gt.
+Proof.
+  intros. unfold Extendcheck. unfold Extendcheck_f in H.
+  intros. apply extf_zero_implies_ext_zero. apply H.
+Qed.
+
+Theorem ECheck_f_imp_ECheck_one : forall (a:assumption) (gt:tguarantee) (s:state),
+Extendcheck_f 1 a gt -> Extendcheck 1 a gt.
+Proof.
+  intros. unfold Extendcheck. unfold Extendcheck_f in H.
+  intros. apply extf_one_implies_ext_one. apply H.
+Qed.
+
+(*Random Notes Below --- Safe to ignore! *)
+
+(*
+
+Inductive extendable_f : nat -> assumption -> tguarantee -> Prop :=
+|exnill : forall sl s (a:assumption) (gt:tguarantee), (sl = scons s snil) /\ (forall i, a s i -> (gt s i (skolem s i))) ->
+extendable_f O sl a gt
+|exone : forall sl s s' (a:assumption) (gt:tguarantee), extendable_f O sl a gt /\ (forall i, a s' i -> gt s i (skolem
+
+
+
+
+Fixpoint extendable_f (n:nat) (s:state) (a:assumption) (gt:tguarantee) : Prop :=
+  match n with
+  | O => forall i, a s i -> gt s i (skolem_0 s i)
+  | S O => forall (i:inputs) s', a s i  /\ s' = skolem_0 s i -> gt s i (skolem s i) -> extendable_f n' s' a gt
+  end.
+
+
+
+Theorem extf_zero_implies_ext_zero : forall (a:assumption) (gt:tguarantee) (s:state),
+extendable_f O s a gt -> extendable O s a gt.
+Proof.
+  intros n a gt.
+  intros. inversion H. simpl. intros. exists (skolem_0 s i).
+  apply H0. apply H1.
+Qed.
+
+Theorem extf_one_implies_ext_one : forall (a:assumption) (gt:tguarantee) (s:state),
+extendable_f 1 s a gt -> extendable 1 s a gt.
+Proof.
+  intros. simpl. intros. simpl in H.
+
+ simpl in H1. intros. 
+  apply H1 in H2. exists (skolem s i). apply H2.
+
+  intros. simpl. inversion H. intros. apply IHn.
+  split. apply H0. simpl in H1. apply H1 with (i:=i).
+  split. apply H2. apply H0. assert (H4: s' = skolem s i).
+  apply H0. rewrite H4 in H3. apply H3.
+Qed.
+
+Definition Basecheck_simple_f_zero (n:nat) (a:assumption) (gi:iguarantee) (gt:tguarantee):=
+forall s, (gi s) -> extendable_f O s a gt.
+
+Definition Basecheck_simple_f_one (n:nat) (a:assumption) (gi:iguarantee) (gt:tguarantee):=
+forall s, (gi s) -> extendable_f 1 s a gt.
+
+Definition Extendcheck_f_zero (n:nat) (a:assumption) (gt:tguarantee) :=
+forall s a gt, extendable_f O s a gt.
+
+Definition Extendcheck_f_one (n:nat) (a:assumption) (gt:tguarantee) :=
+forall s a gt, extendable_f 1 s a gt.
+
+Theorem BCheck_f_imp_BCheck : forall (n:nat) (a:assumption) (gi:iguarantee) (gt:tguarantee) (sl:statelist),
+Basecheck_simple_f O a gi gt -> Basecheck_simple O a gi gt.
+Proof.
+  intros. unfold Basecheck_simple_f in H. unfold Basecheck_simple.
+  intros. apply exs_imp_ex_one. apply sl. apply H. apply H0.
+Qed.
+
+
+
+Inductive statelist : Type :=
+|snil : statelist
+|scons : state -> statelist -> statelist.
+
+Inductive extendable_f : nat -> statelist -> assumption -> tguarantee -> Prop :=
+
+|exnill : forall sl s (a:assumption) (gt:tguarantee), (sl = scons s snil) /\ (forall i, a s i -> (gt s i (skolem s i))) ->
+extendable_f O sl a gt
+|exone : forall sl s s' (a:assumption) (gt:tguarantee), extendable_f O sl a gt /\ (forall i, a s' i -> gt s i (skolem
+|exind : forall m sl a gt i s sl', ((sl = scons s sl') /\ a s i /\ gt s i (skolem s i) /\ extendable_f m sl a gt) -> extendable_f (S m) (scons (skolem s i) sl) a gt.
+
+
+
+Inductive statelist : Type :=
+|snil : statelist
+|scons : state -> inputs -> statelist -> statelist.
+
+
+
+Definition skolem (s:state) (i:inputs) : state := admit.
+
+
+Fixpoint extendable_f (n:nat) (s:state) (a:assumption) (gt:tguarantee) : Prop :=
+  match n with
+  | O => forall i, a s i -> gt s i (skolem s i)
+  | S n' => forall (i:inputs) s', a s i  /\ s' = skolem s i -> gt s i (skolem s i) -> extendable_f n' s' a gt
+  end.
+
+Fixpoint finite_viable_f (n:nat) (s:state) (a:assumption) (gt:tguarantee) : Prop :=
+  match n with
+  | O => True
+  | S n' => forall i, a s i -> gt s i (skolem s i) /\ finite_viable_f n' (skolem s i) a gt
+  end.
+
+
+CoInductive viable_f (s:state) (a:assumption) (gi:iguarantee) (gt: tguarantee) : Prop :=
+vblf : (forall (i:inputs), a s i -> gt s i (skolem s i) /\ viable_f (skolem s i) a gi gt) -> viable_f s a gi gt.
+
+
+Theorem viable_f_implies_viable : forall s a gi gt,
+(viable_f s a gi gt -> viable s a gi gt).
+Proof. cofix.
+  intros. inversion H. apply vbl. intros. apply H0 in H1.
+  exists (skolem s i). inversion H1. split. apply H2. apply viable_f_implies_viable.
+  apply H3.
+Qed.
+
+Definition Basecheck_simple_f (n:nat) (a:assumption) (gi:iguarantee) (gt:tguarantee):=
+forall s, (gi s) -> extendable_f n s a gt.
+
+Definition Extendcheck_f (n:nat) (a:assumption) (gt:tguarantee) :=
+forall s a gt, extendable_f n s a gt.
+
+
+Theorem exs_imp_ex_one : forall (n:nat)  (a:assumption) (gt:tguarantee) (s:state),
+(forall s' i' s'', s'' = skolem s' i') /\ extendable_f n s a gt -> extendable n s a gt.
+Proof.
+  intros n a gt. induction n.
+  intros. inversion H. simpl. simpl in H1. intros. 
+  apply H1 in H2. exists (skolem s i). apply H2.
+
+  intros. simpl. inversion H. intros. apply IHn.
+  split. apply H0. simpl in H1. apply H1 with (i:=i).
+  split. apply H2. apply H0. assert (H4: s' = skolem s i).
+  apply H0. rewrite H4 in H3. apply H3.
+Qed.
+
+Lemma finite_viable_plus_one_f : forall n a gt (gi:iguarantee) (i:inputs) s,
+(forall s' i' s'', s'' = skolem s' i') /\ extendable_f n s a gt /\ finite_viable_f n s a gt -> finite_viable_f (S n) s a gt.
+Proof.
+  intros n a gt gi i. induction n. intros.
+  simpl. intros. inversion H. split. inversion H2. simpl in H3. apply H3.
+  apply H0. auto.
+
+  intros. inversion H. inversion H1. simpl in H2. simpl in H3.
+  simpl. intros. assert (H5: a s i0). apply H4.
+  assert (s':state). apply s. assert (H6: s' = skolem s i0).  
+  apply H0. split. apply conj with (A:=a s i0) in H6. apply H2 in H6.
+  apply H3 in H4. inversion H4. apply H7.
+  apply H3 in H4. inversion H4. apply H7.
+  apply H4.
+  intros. assert (s' = skolem s i0). apply H0.
+  apply conj with (A:=a s i0) in H6. apply H2 in H6.
+  rewrite H8 in H6. apply H3 in H4. inversion H4. 
+  assert (H11:finite_viable_f (S n) (skolem s i0) a gt). 
+  apply IHn. split. apply H0. split. apply H6. apply H10.
+  admit. admit. assumption. Qed.
+
+
+
+Theorem extendable_f_imp_viable_f : forall  (n:nat) (a:assumption) (gi:iguarantee) (gt:tguarantee) (s:state),
+(forall i, a s i /\ finite_viable_f n s a gt /\ Extendcheck_f n a gt) -> viable_f s a gi gt.
+Proof.
+  cofix. intros n a gi gt. induction n.
+  intros. apply vblf. intros. split. assert (H1: a s i /\ finite_viable_f 0 s a gt /\ Extendcheck_f 0 a gt).
+  apply H. inversion H1. inversion H3. unfold Extendcheck_f in H5. assert (H6: extendable_f 0 s a gt).
+  apply H5. simpl in H6. apply H6. apply H2. admit. admit.
+Qed.
+
+
+Inductive statelist : Type :=
+|snil : statelist
+|scons : state -> inputs -> statelist -> statelist.
+ 
+
+Fixpoint skolem (s:state) (i:inputs) (sl:statelist) (a:assumption) (gt:tguarantee): Prop := 
+  match sl with
+  |snil => a s i /\ exists s':state, gt s i s'
+  |scons s' i' sl' => a s' i' -> gt s' i' s -> a s i -> exists s'', gt s i s'' -> skolem s' i' sl' a gt
+  end.
+
+
+
+Fixpoint extendable_f (n:nat) (s:state) (a:assumption) (gt:tguarantee): Prop :=
+  match n with
+  | O => forall i sl, a s i -> skolem s i sl a gt
+  | S n' => forall i sl s', skolem s i sl a gt -> gt s i s' -> extendable_f n' s' a gt
+  end.
+
+Fixpoint finite_viable_f (n:nat) (s:state) (a:assumption) (gt:tguarantee) : Prop :=
+  match n with
+  | O => True
+  | S n' => forall i sl, a s i -> exists s', skolem s i sl a gt -> gt s i s' /\ finite_viable_f n' s' a gt
+  end.
+
+
+CoInductive viable_f (s:state) (a:assumption) (gi:iguarantee) (gt: tguarantee) : Prop :=
+vblf : (forall (i:inputs) (sl:statelist) s', a s i -> skolem s i sl a gt /\ gt s i s' /\ viable_f s' a gi gt) -> viable_f s a gi gt.
+
+Theorem viable_f_implies_viable : forall s a gi gt (sl:statelist),
+(viable_f s a gi gt -> viable s a gi gt).
+Proof. cofix.
+  intros. inversion H. apply vbl. intros. assert (x:state). apply s.
+  destruct H0 with (i:=i) (sl:=sl) (s':=x). apply H1. inversion H3. exists x.
+  split. apply H4. apply viable_f_implies_viable. apply sl. apply H5.
+Qed.
+
+
+Definition Basecheck_simple_f (n:nat) (a:assumption) (gi:iguarantee) (gt:tguarantee):=
+forall s, (gi s) -> extendable_f n s a gt.
+
+Definition Extendcheck_f (n:nat) (a:assumption) (gt:tguarantee) :=
+forall s a gt, extendable_f n s a gt.
+
+Theorem exs_imp_ex_one : forall (n:nat)  (a:assumption) (gt:tguarantee) (sl:statelist) (s:state),
+extendable_f n s a gt -> extendable n s a gt.
+Proof.
+  intros n a gt sl. induction n. induction sl. intros.
+  simpl. intros. simpl in H. apply H with (sl:=snil) in H0.
+  simpl in H0. inversion H0. inversion H2. exists x. apply H3.  
+  intros. apply IHsl. apply H.
+
+  induction sl. intros. simpl. intros. apply IHn. simpl in H. apply H with (i:=i) (sl:=snil).
+  simpl. split. apply H0. exists s'. apply H1. apply H1.
+  intros. apply IHsl. apply H.
+Qed.
+
+Theorem BCheck_f_imp_BCheck : forall (n:nat) (a:assumption) (gi:iguarantee) (gt:tguarantee) (sl:statelist),
+Basecheck_simple_f n a gi gt -> Basecheck_simple n a gi gt.
+Proof.
+  intros. unfold Basecheck_simple_f in H. unfold Basecheck_simple.
+  intros. apply exs_imp_ex_one. apply sl. apply H. apply H0.
+Qed.
+
+Theorem ECheck_f_imp_ECheck : forall (n:nat) (a:assumption) (gt:tguarantee) (sl:statelist) (s:state) (sl:statelist),
+Extendcheck_f n a gt -> Extendcheck n a gt.
+Proof.
+  intros. unfold Extendcheck. unfold Extendcheck_f in H.
+  intros. apply exs_imp_ex_one. apply sl. apply H.
+Qed.
+
+
+Theorem extendable_f_imp_viable_f : forall  (n:nat) (a:assumption) (gi:iguarantee) (gt:tguarantee) (s:state),
+(forall i, a s i /\ finite_viable_f n s a gt /\ Extendcheck_f n a gt) -> viable_f s a gi gt.
+Proof.
+  cofix. intros. apply vblf. intros.
+  destruct H with (i:=i). unfold Extendcheck_f in H2. inversion H2.
+  assert (H4: extendable_f n s a gt). apply H3. induction n. simpl in H4.
+  apply H4 with (sl:=sl) in H0. split. apply H0. split. induction sl.
+  simpl in H0. inversion H0. apply H6.
+ assert (H4: extendable_f 0 s a gt).
+  apply H1. simpl in H4. split. apply H4. apply H4 in 
+ cofix. intros. apply vblf. induction n.
+  intros. split.
+
+
+
+
+
+
+
+
+ induction intros. inversion H. assert (H10: a s i). assumption. apply conj with (A:=finite_viable_f 0 s a gt) in H0.
+ unfold Extendcheck_f in H2. assert (H3: extendable_f 0 s a gt). apply H2. apply conj with (A:= extendable_f 0 s a gt) in H0.
+ apply extend_f_viable_f_shift in H0. inversion H3. apply H4 in H10. apply if_skolem_then_gt_holds in H10. 
+ inversion H10.  exists x. split.  inversion H5. assumption. split. inversion H5. assumption.
+ apply extendable_f_imp_viable_f. split. apply fvnill. unfold Extendcheck_f.
+ intros. apply H2. assumption. assumption. assumption. assumption.
+Qed.
+
+
+Lemma extend_f_viable_f_shift : forall (n:nat) (a:assumption) (gi:iguarantee) (gt:tguarantee) (s:state) (i:inputs),
+(extendable_f n s a gt /\ finite_viable_f n s a gt /\ a s i) -> forall i' (sl:statelist), exists s', (skolem s' i' (scons s i sl) a gt) /\ finite_viable_f n s' a gt.
+Proof.
+  intros n a gi gt. induction n.
+  intros. inversion H. simpl in H0. 
+  inversion H1. apply H0 with (sl:=sl) in H3.
+  induction sl. simpl in H3. inversion H3. inversion H5.
+  exists x. split. simpl. intros. assert (s'':state).
+  apply s. exists s''. intros. split. apply H4. exists x. apply H6.
+  simpl. auto.
+
+  apply IHsl.
+ simpl in H0. inversion H1. 
+  apply H0 with(sl:=snil) in H3. simpl in H3.
+  inversion H3. inversion H5. exists x. intros.
+  split. simpl. intros. assert (s'':state). apply s.
+  exists s''. intros. apply H3. simpl. auto.
+
+  intros. apply IHsl in H. inversion H. exists x. intros.
+  simpl. intros. split. intros. assert (s'':state). apply s. 
+  exists s''. intros.
+ split. simpl. intros. intros.
+ split. inversion H. simpl in H0.(sl:statelist) 
+  simpl.
+  induction sl. simpl.
+  simpl. split. split. inversion H1. apply H3. split.
+  assert (H2: skolem s i sl a gt). apply H0. inversion H1. apply H3.
+  induction sl. simpl in H2.  inversion H2.
+  simpl in H2. apply H0 with (sl:=(scons s i sl)). inversion H1. apply H3. simpl. auto.
+  
+  intros. split. simpl. split.
+  inversion H. simpl in H0. inversion H1. simpl in H2. apply H2 with (s':=s') (sl:=sl) in H3.
+  assert (H4: skolem s i (scons s' i' sl) a gt /\ finite_viable_f n s' a gt).
+  apply H0.
+  apply IHn. inversion H. simpl in H0.
+  assert (H2: skolem s i sl a gt /\ gt s i s' /\ extendable_f n s a gt).
+  apply H0.
+  
+
+
+
+ inversion H. inversion H1. exists s.
+  inversion H0. apply H2. inversion H1. apply H8.
+  apply IHn. split. inversion H. inversion H2. inversion H5.
+  apply H10. split. inversion H1. inversion H2. apply H5.
+  inversion H1. apply H3. inversion H0. inversion H3. apply H8.
+  inversion H1. inversion H2. split. apply H5. apply H3.
+
+  induction n. apply fvnill. apply fvv. apply IHn. inversion H0.
+  inversion H3. split. apply H8. split. inversion H. inversion H11.
+  inversion H12. apply H15. inversion H1. apply H11.
+  inversion H0. inversion H3. apply H8. inversion H1.
+  inversion H2. split. apply H5. apply H3.
+  intros. inversion H0. inversion H4.
+  assert (H12: compatible_f sl s i a gt /\ gt (extendable_f 0 (skolem (hds s sl) (hdi i sl) sl) sl a gt).
+  inversion H4. apply H10. inversion H12. inversion H10. apply H11. inversion H9.
+   inversion H11. destruct H10.
+
+apply fvv.
+
+ inversion H0. inversion H1. split. 
+  apply H2. apply H9. apply fvnill.
+  split. 
+  split.  inversion H2. inversion H8. apply H10. inversion H1. apply H17.
+apply H2 in H7. apply if_skolem_then_gt_holds in H7.
+  inversion H7. exists x. inversion H8. split. assumption. apply fvv. assumption. assumption. assumption.
+Qed.
+
+
+Theorem extendable_f_imp_viable_f : forall (s:state) (a:assumption) (gi:iguarantee) (gt:tguarantee),
+(finite_viable_f O s a gt /\ Extendcheck_f O a gt) -> viable_f s a gi gt.
+Proof.
+ cofix. intros. apply vblf. intros. inversion H. assert (H10: a s i). assumption. apply conj with (A:=finite_viable_f 0 s a gt) in H0.
+ unfold Extendcheck_f in H2. assert (H3: extendable_f 0 s a gt). apply H2. apply conj with (A:= extendable_f 0 s a gt) in H0.
+ apply extend_f_viable_f_shift in H0. inversion H3. apply H4 in H10. apply if_skolem_then_gt_holds in H10. 
+ inversion H10.  exists x. split.  inversion H5. assumption. split. inversion H5. assumption.
+ apply extendable_f_imp_viable_f. split. apply fvnill. unfold Extendcheck_f.
+ intros. apply H2. assumption. assumption. assumption. assumption.
+Qed.
+*)
